SyBloc/SBIsFree.v
@@ -41,6 +41,51 @@ Module Type SBISFREE
   Definition Is_free_in (x: ident) (eqs: list equation) : Prop :=
     Exists (Is_free_in_eq x) eqs.
 
+  Definition free_in_eq (eq: equation) (fvs: PS.t) : PS.t :=
+    match eq with
+    | EqDef _ ck e => free_in_caexp ck e fvs
+    | EqNext _ ck e => free_in_laexp ck e fvs
+    | EqReset _ ck _ => free_in_clock ck fvs
+    | EqCall _ _ ck _ _ es => free_in_laexps ck es fvs
+    end.
+
+  Hint Constructors Is_free_in_clock Is_free_in_lexp
+       Is_free_in_laexp Is_free_in_laexps Is_free_in_cexp
+       Is_free_in_caexp Is_free_in_eq.
+
+  Lemma free_in_eq_spec:
+    forall x eq m,
+      PS.In x (free_in_eq eq m)
+      <-> (Is_free_in_eq x eq \/ PS.In x m).
+  Proof.
+    Local Ltac aux :=
+      repeat (match goal with
+              | H:Is_free_in_eq _ _ |- _ => inversion_clear H
+              | H:PS.In _ (free_in_eq _ _) |- _ =>
+                apply free_in_clock_spec in H
+                || apply free_in_caexp_spec in H
+                || apply free_in_laexp_spec in H
+                || apply free_in_laexps_spec in H
+              | |- PS.In _ (free_in_eq _ _) =>
+                apply free_in_clock_spec
+                || apply free_in_caexp_spec
+                || apply free_in_laexp_spec
+                || apply free_in_laexps_spec
+              | _ => intuition; eauto
+              end).
+    destruct eq; split; intro H; aux.
+  Qed.
+
+  Corollary free_in_eq_spec':
+    forall x eq,
+      PS.In x (free_in_eq eq PS.empty)
+      <-> Is_free_in_eq x eq.
+  Proof.
+    intros; rewrite free_in_eq_spec.
+    intuition not_In_empty.
+  Qed.
+
+
 End SBISFREE.
 
 Module SBIsFreeFun
