SyBloc/SBWellDefined.v
@@ -207,6 +207,430 @@ Module Type SBWELLDEFINED
       + intro; apply Step; right; auto.
   Qed.
 
+  Section Decide.
+
+    Variable mems : PS.t.
+
+    (* TODO: rewrite using a strong specification?  *)
+
+    Open Scope bool_scope.
+
+    Definition check_var (defined: PS.t) (variables: PS.t) (x: ident) : bool :=
+      if PS.mem x mems
+      then negb (PS.mem x defined)
+      else PS.mem x variables.
+
+    Lemma check_var_spec:
+      forall defined variables x,
+        check_var defined variables x = true
+        <->
+        (PS.In x mems -> ~PS.In x defined)
+        /\ (~PS.In x mems -> PS.In x variables).
+    Proof.
+      (*  TODO: how to automate all of this? *)
+      intros defined variables x.
+      unfold check_var.
+      split.
+      - intro Hif.
+        split; intro Hin.
+        + apply PS.mem_spec in Hin.
+          rewrite Hin, Bool.negb_true_iff in Hif.
+          apply mem_spec_false in Hif. exact Hif.
+        + apply mem_spec_false in Hin.
+          rewrite Hin, PS.mem_spec in Hif. exact Hif.
+      - destruct 1 as [Hin Hnin].
+        destruct PSP.In_dec with x mems as [H|H].
+        + assert (PS.mem x mems = true) as H' by auto.
+          rewrite H', Bool.negb_true_iff, mem_spec_false.
+          now apply Hin with (1:=H).
+        + assert (PS.mem x mems = false) as H' by now apply mem_spec_false.
+          rewrite H', PS.mem_spec.
+          now apply Hnin with (1:=H).
+    Qed.
+
+    Definition state_eq (eq: equation) : option (ident * nat) :=
+      match eq with
+      | EqReset s _ _ => Some (s, 0)
+      | EqCall s _ _ _ _ _ => Some (s, 1)
+      | _ => None
+      end.
+
+    Lemma Is_state_in_state_eq:
+      forall eq s k,
+        Is_state_in_eq s k eq <-> state_eq eq = Some (s, k).
+    Proof.
+      destruct eq; simpl; split; try inversion_clear 1; auto using Is_state_in_eq.
+    Qed.
+
+    Definition check_eq (eq: equation) (acc: bool * PS.t * PS.t * Env.t nat) : bool * PS.t * PS.t * Env.t nat :=
+      match acc with
+      | (true, defs, vars, states) =>
+        let xs := defined_eq eq in
+        let b := PS.for_all (check_var defs vars) (free_in_eq eq PS.empty)
+                            && negb (existsb (fun x => PS.mem x defs) xs) in
+        let defs := ps_adds xs defs in
+        let vars := variables_eq vars eq in
+        match state_eq eq with
+        | Some (s, k) =>
+          (match Env.find s states with
+           | Some k' => NPeano.ltb k' k && b
+           | None => b
+           end,
+           defs, vars, Env.add s k states)
+        | None => (b, defs, vars, states)
+        end
+      | (false, _, _, _) => (false, PS.empty, PS.empty, Env.empty _)
+      end.
+
+    Definition well_sch (args: idents) (eqs: list equation) : bool :=
+      fst (fst (fst (fold_right check_eq (true,
+                                          PS.empty,
+                                          ps_from_list args,
+                                          Env.empty _) eqs))).
+
+    Lemma not_for_all_spec:
+      forall (s : PS.t) (f : BinNums.positive -> bool),
+        SetoidList.compat_bool PS.E.eq f ->
+        (PS.for_all f s = false <-> ~(PS.For_all (fun x : PS.elt => f x = true) s)).
+    Proof.
+      intros s f HSL.
+      split.
+      - intros Hfa HFa.
+        apply (PS.for_all_spec _ HSL) in HFa.
+        rewrite Hfa in HFa.
+        discriminate.
+      - intro HFa.
+        apply Bool.not_true_iff_false.
+        intro Hfa; apply HFa.
+        apply (PS.for_all_spec _ HSL).
+        assumption.
+    Qed.
+
+    Lemma check_var_compat:
+      forall defined variables,
+        SetoidList.compat_bool PS.E.eq (check_var defined variables).
+    Proof.
+      intros defined variables x y Heq.
+      unfold PS.E.eq in Heq.
+      rewrite Heq.
+      reflexivity.
+    Qed.
+
+    (* Lemma in_fold_left_add: *)
+    (*   forall x xs S, *)
+    (*     PS.In x (fold_left (fun S' x => PS.add x S') xs S) *)
+    (*     <-> *)
+    (*     In x xs \/ PS.In x S. *)
+    (* Proof. *)
+    (*   induction xs as [|y xs IH]. *)
+    (*   split; intro H; simpl in *; *)
+    (*     intuition. *)
+    (*   intro S; split; intro H. *)
+    (*   - apply IH in H. *)
+    (*     destruct H. *)
+    (*     now left; constructor (assumption). *)
+    (*     apply PS.add_spec in H; simpl; intuition. *)
+    (*   - simpl; apply IH; simpl in H; intuition. *)
+    (* Qed. *)
+
+    Lemma well_sch_pre_spec:
+      forall args eqs ok defs vars states,
+        fold_right check_eq (true,
+                             PS.empty,
+                             ps_from_list args,
+                             Env.empty _) eqs = (ok, defs, vars, states) ->
+        if ok
+        then
+          Is_well_sch args mems eqs
+          /\ (forall x, PS.In x defs <-> Is_defined_in x eqs)
+          /\ (forall x, PS.In x vars <-> Is_variable_in x eqs \/ In x args)
+          /\ (forall s k, Env.find s states = Some k <-> Is_state_in s k eqs)
+        else
+          ~Is_well_sch args mems eqs.
+    Proof.
+      induction eqs as [|eq].
+      - simpl; inversion_clear 1; intuition; try (now constructor);
+          repeat match goal with
+                 | H:PS.In _ PS.empty |- _ => apply PS.empty_spec in H; contradiction
+                 | H:Env.find _ (Env.empty _) = _ |- _ => rewrite Env.gempty in H; discriminate
+                 | H:Is_defined_in _ nil |- _ => inversion H
+                 | H:Is_variable_in _ nil |- _ => inversion H
+                 | H:Is_state_in _ _ nil |- _ => inversion H
+                 | H: context[ps_from_list _] |- _ =>
+                   apply ps_from_list_In in H
+                 | _ => intuition
+                 end.
+        apply ps_from_list_In; auto.
+      - simpl; intros ** HH.
+        destruct (fold_right check_eq (true, PS.empty, ps_from_list args, Env.empty nat) eqs)
+          as [[[ok' defs'] vars'] states'].
+        specialize (IHeqs ok' defs'  vars' states' eq_refl).
+        simpl in HH.
+        destruct ok'.
+        + destruct IHeqs as (Wsch & DefSpec & VarSpec & StateSpec).
+          destruct (state_eq eq) eqn: St.
+          * admit.
+          *{ destruct ok; inversion HH as [E]; [apply Bool.andb_true_iff in E as (E & E')|].
+             - apply PS.for_all_spec in E; try now apply check_var_compat.
+               apply Bool.negb_true_iff in E'.
+               split; [|split; [|split]].
+               + constructor; auto.
+                 *{ intros ** Hfree.
+                    apply free_in_eq_spec', E, check_var_spec in Hfree as (Hin & Hnin).
+                    destruct (PS.mem x mems) eqn: Mem.
+                    - rewrite <-DefSpec; apply PSE.MP.Dec.F.mem_iff, Hin in Mem; auto.
+                    - rewrite <-VarSpec; apply PSE.MP.Dec.F.not_mem_iff, Hnin in Mem; auto.
+                  }
+                 * setoid_rewrite <-DefSpec; setoid_rewrite Is_defined_in_defined_eq.
+                   intros x Hin.
+                   apply In_ex_nth with (d := Ids.default) in Hin as (?&?&?); subst.
+                   eapply existsb_nth with (d := Ids.default) in E'; eauto.
+                   now apply PSE.MP.Dec.F.not_mem_iff.
+                 * setoid_rewrite Is_state_in_state_eq; rewrite St; discriminate.
+               + intro x; split; intro Hin;
+                   [apply ps_adds_spec in Hin as [|]|apply ps_adds_spec; inv Hin];
+                   try (now left; apply Is_defined_in_defined_eq; auto);
+                   try (now right; apply DefSpec; auto); auto.
+               + intro x; split; intro Hin.
+                 *
+                 (* variables set *)
+            intro x; split; intro HH.
+            apply variable_eq_empty in HH.
+            destruct HH as [HH|HH].
+            destruct eq;
+              match goal with
+              | |- context[ EqApp _ _ _ _ ] =>
+                generalize ps_adds_spec; intro add_spec
+              | _ =>
+                generalize PS.add_spec; intro add_spec
+              end;
+              ((apply add_spec in HH;
+                destruct HH as [HH|HH];
+                [try subst i; left; now repeat constructor
+                |apply PS.empty_spec in HH; contradiction])
+               || apply PS.empty_spec in HH; contradiction).
+            apply IHvar in HH; intuition; left; constructor (assumption).
+            apply variable_eq_empty.
+            destruct HH as [HH|HH].
+            apply Is_variable_in_cons in HH.
+            destruct HH as [HH|HH]; [left|right].
+            destruct eq;
+              match goal with
+              | |- context[ EqApp _ _ _ _ ] =>
+                generalize ps_adds_spec; intro add_spec
+              | _ =>
+                generalize PS.add_spec; intro add_spec
+              end;
+              inversion_clear HH; simpl;
+                try (rewrite add_spec; auto);
+                intuition.
+            apply IHvar; intuition.
+            right; apply IHvar; auto.
+
+               SearchAbout (_ && _) true. inv HH.
+
+        + inv HH.
+          inversion_clear 1; contradiction.
+
+
+
+
+          simpl in HH.
+        destruct IH as [IHt IHf].
+        split; intro Hg; rewrite Hg in *; clear Hg.
+        + (* good=true *)
+          simpl in HH; rewrite Heq in HH.
+          simpl in HH.
+          destruct good'; [|discriminate].
+          specialize (IHt eq_refl).
+          clear IHf; destruct IHt as [IHwsch [IHdef IHvar]].
+          injection HH; clear HH; intros Hv Hd H.
+          subst variables; subst defined.
+          symmetry in H.
+          apply Bool.andb_true_iff in H.
+          destruct H as [H1 H2].
+          apply PS.for_all_spec in H1; [|now apply check_var_compat].
+          apply Bool.negb_true_iff in H2.
+
+          assert (forall x, In x (var_defined eq) -> ~ PS.In x defined')
+            as Hnot_def.
+          {
+            intros x Hin.
+
+            assert (exists n,
+                       n < length (var_defined eq)
+                     /\ nth n (var_defined eq) Ids.default = x)
+              as (n & Hlen & Hnth)
+                by now apply In_ex_nth.
+
+            assert (PS.mem x defined' = false)
+              by now subst x;
+                     eapply existsb_nth
+                       with (f := (fun x => PS.mem x defined')).
+
+            now apply mem_spec_false.
+          }
+
+          split; [|split].
+          * (* Is_well_sch *)
+            assert (forall i,
+                       IsF.Is_free_in_eq i eq ->
+                       (PS.In i mems -> ~ Is_defined_in_eqs i eqs) /\
+                       (~ PS.In i mems -> Is_variable_in_eqs i eqs \/ In i args)).
+            {
+              intros x Hfree.
+              apply free_in_equation_spec' in Hfree.
+              apply H1 in Hfree.
+              apply check_var_spec in Hfree.
+              destruct Hfree as [Hfree1 Hfree2].
+              split; intro HH; (apply Hfree1 in HH || apply Hfree2 in HH).
+              - now intro; apply HH; apply IHdef.
+              - now apply IHvar.
+            }
+
+            assert (forall i, Is_defined_in_eq i eq -> ~ Is_defined_in_eqs i eqs).
+            {
+              intros x Hdef Hdefs; apply IHdef in Hdefs.
+              apply Is_defined_in_eqs_var_defined in Hdef.
+              now eapply Hnot_def; eauto.
+            }
+
+            now constructor.
+          * (* defined set *)
+            intro x; split; intro HH.
+            apply ps_adds_spec in HH.
+            destruct HH as [HH|HH].
+            constructor; now apply Is_defined_in_eqs_var_defined.
+            apply IHdef in HH.
+            constructor (assumption).
+            apply ps_adds_spec.
+            inversion_clear HH.
+            apply Is_defined_in_eqs_var_defined in H; auto.
+            right; apply IHdef; assumption.
+          * (* variables set *)
+            intro x; split; intro HH.
+            apply variable_eq_empty in HH.
+            destruct HH as [HH|HH].
+            destruct eq;
+              match goal with
+              | |- context[ EqApp _ _ _ _ ] =>
+                generalize ps_adds_spec; intro add_spec
+              | _ =>
+                generalize PS.add_spec; intro add_spec
+              end;
+              ((apply add_spec in HH;
+                destruct HH as [HH|HH];
+                [try subst i; left; now repeat constructor
+                |apply PS.empty_spec in HH; contradiction])
+               || apply PS.empty_spec in HH; contradiction).
+            apply IHvar in HH; intuition; left; constructor (assumption).
+            apply variable_eq_empty.
+            destruct HH as [HH|HH].
+            apply Is_variable_in_cons in HH.
+            destruct HH as [HH|HH]; [left|right].
+            destruct eq;
+              match goal with
+              | |- context[ EqApp _ _ _ _ ] =>
+                generalize ps_adds_spec; intro add_spec
+              | _ =>
+                generalize PS.add_spec; intro add_spec
+              end;
+              inversion_clear HH; simpl;
+                try (rewrite add_spec; auto);
+                intuition.
+            apply IHvar; intuition.
+            right; apply IHvar; auto.
+        + (* good=false *)
+          intro Hwsch.
+          simpl in HH; rewrite Heq in HH; clear Heq; simpl in HH.
+          destruct good'; [specialize (IHt eq_refl); clear IHf
+                          | specialize (IHf eq_refl);
+                            apply Is_well_sch_cons in Hwsch;
+                            apply IHf with (1:=Hwsch)].
+          destruct IHt as [_ [IHdef IHvar]].
+          injection HH; clear HH; intros Hv Hd HH.
+          subst variables; subst defined; symmetry in HH.
+          apply Bool.andb_false_iff in HH.
+          inversion_clear Hwsch as [|Ha Hb Hwschs Hfree Hdefd].
+          destruct HH as [HH|HH].
+          * (* check_var of free fails *)
+            apply not_for_all_spec in HH; [|apply check_var_compat].
+            apply HH; clear HH.
+            intros x HH.
+            apply free_in_equation_spec in HH.
+            destruct HH as [HH|HH]; [|apply PS.empty_spec in HH].
+            apply Hfree in HH.
+            destruct HH as [Hmem Hvar];
+              apply check_var_spec; split; intro HHm;
+                (specialize (Hmem HHm) || specialize (Hvar HHm)).
+            intro Hdef; apply IHdef in Hdef; apply Hmem; assumption.
+            apply IHvar; intuition.
+            contradiction.
+          * (* already defined *)
+            apply Bool.negb_false_iff in HH.
+
+            assert (exists x, In x (var_defined eq) /\ PS.In x defined')
+              as (x & Hdef & Hdef').
+            {
+              apply existsb_exists in HH.
+              destruct HH as (x & Hvar_def & Hmem).
+              rewrite PS.mem_spec in Hmem.
+              now eexists; eauto.
+            }
+
+            assert (Is_defined_in_eq x eq)
+              by now apply Is_defined_in_eqs_var_defined.
+
+            assert (Is_defined_in_eqs x eqs)
+              by now apply IHdef.
+
+            eapply Hdefd; now eauto.
+    Qed.
+
+    Lemma well_sch_spec:
+      forall args eqns,
+        if well_sch args eqns
+        then Is_well_sch mems args eqns
+        else ~Is_well_sch mems args eqns.
+    Proof.
+      intros args eqns.
+      pose proof (well_sch_pre_spec args eqns).
+      unfold well_sch.
+      destruct (fold_right check_eq
+                  (true, PS.empty,
+                   fold_left (fun a b => PS.add b a) args PS.empty) eqns)
+        as [[good defined] variables].
+      simpl.
+      specialize H with good defined variables.
+      pose proof (H (eq_refl _)) as H'; clear H.
+      destruct H' as [Ht Hf].
+      destruct good;
+        intuition.
+    Qed.
+
+    Lemma Is_well_sch_by_refl:
+      forall args eqns,
+        well_sch args eqns = true <-> Is_well_sch mems args eqns.
+    Proof.
+      intros args eqns.
+      pose proof (well_sch_spec args eqns) as Hwss.
+      split; intro H.
+      rewrite H in Hwss; assumption.
+      destruct (well_sch args eqns); [reflexivity|].
+      exfalso; apply Hwss; apply H.
+    Qed.
+
+    Lemma well_sch_dec:
+      forall args eqns,
+        {Is_well_sch mems args eqns}+{~Is_well_sch mems args eqns}.
+    Proof.
+      intros args eqns.
+      pose proof (well_sch_spec args eqns) as Hwss.
+      destruct (well_sch args eqns); [left|right]; assumption.
+    Qed.
+
+  End Decide.
+
 End SBWELLDEFINED.
 
 Module SBWellDefinedFun
