NLustreToSyBloc/Correctness.v
@@ -737,31 +737,31 @@ Module Type CORRECTNESS
   (*   - intro; subst; eapply msem_node_initial_state; eauto. *)
   (*   - apply correctness; eauto. *)
   (*   - SearchAbout msem_node. eapply COFIX.  SearchAbout initial_state. *)
-  Theorem correctness_dostep:
-    forall G f xss M M' yss,
-      Ordered_nodes G ->
-      wc_global G ->
-      msem_node G f xss M M' yss ->
-      dostep (translate G) f xss yss (M 0) 0.
-  Proof.
-    (* intros; apply dostep_coind with (R := fun P b xss yss S n => *)
-    (*                                         P = translate G *)
-    (*                                         /\ S = M n  *)
-    (*                                         /\ msem_node G b xss M M' yss); auto. *)
-    (* intros ** (?&?& Sem); subst. *)
-    (* split. *)
-    (* - intro; subst; eapply msem_node_initial_state; eauto. *)
-    (* - pose proof Sem. apply correctness in Sem; auto. *)
-    (*   exists (M' n); intuition. intros ** (?&?). intuition. *)
-    (*   exists (M' n); intuition. *)
-    generalize 0.
-    cofix COFIX; intros ** Sem.
-    econstructor.
-    - intro; subst; eapply msem_node_initial_state; eauto.
-    - apply correctness; eauto.
-    - assert (M' n = M (S n)) as -> by admit.
-      eapply COFIX; eauto.
-  Qed.
+  (* Theorem correctness_dostep: *)
+  (*   forall G f xss M M' yss, *)
+  (*     Ordered_nodes G -> *)
+  (*     wc_global G -> *)
+  (*     msem_node G f xss M M' yss -> *)
+  (*     dostep (translate G) f xss yss (M 0) 0. *)
+  (* Proof. *)
+  (*   (* intros; apply dostep_coind with (R := fun P b xss yss S n => *) *)
+  (*   (*                                         P = translate G *) *)
+  (*   (*                                         /\ S = M n  *) *)
+  (*   (*                                         /\ msem_node G b xss M M' yss); auto. *) *)
+  (*   (* intros ** (?&?& Sem); subst. *) *)
+  (*   (* split. *) *)
+  (*   (* - intro; subst; eapply msem_node_initial_state; eauto. *) *)
+  (*   (* - pose proof Sem. apply correctness in Sem; auto. *) *)
+  (*   (*   exists (M' n); intuition. intros ** (?&?). intuition. *) *)
+  (*   (*   exists (M' n); intuition. *) *)
+  (*   generalize 0. *)
+  (*   cofix COFIX; intros ** Sem. *)
+  (*   econstructor. *)
+  (*   - intro; subst; eapply msem_node_initial_state; eauto. *)
+  (*   - apply correctness; eauto. *)
+  (*   - assert (M' n = M (S n)) as -> by admit. *)
+  (*     eapply COFIX; eauto. *)
+  (* Qed. *)
 
 End CORRECTNESS.
 
